start updating decProps

compiler/backend/semantics/decPropsScript.sml
@@ -2,46 +2,46 @@ open preamble decSemTheory;
 
 val _ = new_theory"decProps"
 
-val csg_rel_def = Define`
-  csg_rel R ((c1,s1),g1) (((c2,s2),g2):('ffi,'v) count_store_genv) ⇔
-    c1 = c2 ∧ LIST_REL (sv_rel R) (FST s1) (FST s2) ∧ (SND s1 = SND s2) ∧ LIST_REL (OPTION_REL R) g1 g2`
+val state_rel_def = Define`
+  state_rel R s1 s2 ⇔
+    s1.clock = s2.clock ∧
+    LIST_REL (sv_rel R) s1.refs s2.refs ∧
+    s1.ffi = s2.ffi ∧
+    LIST_REL (OPTION_REL R) s1.globals s2.globals`;
 
-val csg_rel_refl = store_thm("csg_rel_refl",
-  ``∀V x. (∀x. V x x) ⇒ csg_rel V x x``,
-  rpt gen_tac >> PairCases_on`x` >> simp[csg_rel_def] >>
-  rw[] >> match_mp_tac EVERY2_refl >>
+val state_rel_refl = store_thm("state_rel_refl[simp]",
+  ``∀V s. (∀x. V x x) ⇒ state_rel V s s``,
+  rw[state_rel_def] >>
+  match_mp_tac EVERY2_refl >>
   rw[optionTheory.OPTREL_def] >>
-  Cases_on`x` >> rw[])
-val _ = export_rewrites["csg_rel_refl"]
+  Cases_on`x` >> rw[]);
 
-val csg_rel_trans = store_thm("csg_rel_trans",
-  ``∀V. (∀x y z. V x y ∧ V y z ⇒ V x z) ⇒ ∀x y z. csg_rel V x y ∧ csg_rel V y z ⇒ csg_rel V x z``,
-  rw[] >> map_every PairCases_on [`x`,`y`,`z`] >>
-  fs[csg_rel_def] >>
-  conj_tac >>
+val state_rel_trans = store_thm("csg_rel_trans",
+  ``∀V. (∀x y z. V x y ∧ V y z ⇒ V x z) ⇒ ∀x y z. state_rel V x y ∧ state_rel V y z ⇒ state_rel V x z``,
+  rw[state_rel_def] >>
   match_mp_tac (MP_CANON EVERY2_trans)
   >- metis_tac[evalPropsTheory.sv_rel_trans] >>
   simp[optionTheory.OPTREL_def] >>
-  qexists_tac`y3` >> simp[] >>
-  Cases >> Cases >> Cases >> simp[] >>
+  srw_tac[boolSimps.DNF_ss][] >>
   metis_tac[])
 
-val csg_rel_count = store_thm("csg_rel_count",
-  ``csg_rel R csg1 csg2 ⇒ FST(FST csg2) = FST(FST csg1)``,
-  PairCases_on`csg1` >>
-  PairCases_on`csg2` >>
-  simp[csg_rel_def])
+val state_rel_clock = store_thm("state_rel_clock",
+  ``state_rel R csg1 csg2 ⇒ csg1.clock = csg2.clock``,
+  simp[state_rel_def])
 
-val map_csg_def = Define`
-  map_csg f (csg:('ffi,'v) count_store_genv) =
-    ((FST(FST csg), (MAP (map_sv f) (FST(SND(FST csg))),SND(SND(FST csg)))), MAP (OPTION_MAP f) (SND csg))`
+val map_state_def = Define`
+  map_state f s =
+    <|clock := s.clock;
+      ffi := s.ffi;
+      refs := MAP (map_sv f) s.refs;
+      globals := MAP (OPTION_MAP f) s.globals |>`;
 
-val map_csg_count = Q.store_thm("map_csg_count",
-  `FST(FST (map_csg f csg)) = FST(FST csg)`,
-  PairCases_on`csg`>>simp[map_csg_def])
+val map_state_clock = Q.store_thm("map_state_clock[simp]",
+  `(map_state f s).clock = s.clock`,
+  rw[map_state_def]);
 
-val csg_every_def = Define`
-  csg_every P (((c,s),g):('ffi,'v) count_store_genv) ⇔ EVERY (sv_every P) (FST s) ∧ EVERY (OPTION_EVERY P) g`
+val state_every_def = Define`
+  state_every P s ⇔ EVERY (sv_every P) s.refs ∧ EVERY (OPTION_EVERY P) s.globals`
 
 val do_app_genv_weakening = prove(
   ``decSem$do_app (x,y) op vs = SOME ((a,b),c) ⇒
